src/contracts_coq/did_manager_michelson_string.v
@@ -1,0 +1,33 @@
+Require Import String.
+
+Definition did_manager_michelson_string : string := "
+parameter (or (address %owner) (or (address %auth) (pair %service string string))) ;
+storage
+  (pair (pair (big_map %metadata string bytes) address)
+        (pair (pair string string) address)) ;
+code { UNPAIR ;
+       SWAP ;
+       UNPAIR ;
+       UNPAIR ;
+       SWAP ;
+       DUP ;
+       SENDER ;
+       COMPARE ;
+       EQ ;
+       IF { DIG 3 ;
+            IF_LEFT
+              { SWAP ; DROP ; SWAP }
+              { DIG 3 ;
+                SWAP ;
+                IF_LEFT { SWAP ; CAR } { SWAP ; CDR ; SWAP } ;
+                PAIR ;
+                DUG 2 ;
+                SWAP } ;
+            PUSH mutez 0 ;
+            AMOUNT ;
+            COMPARE ;
+            GT ;
+            IF { SWAP ; FAILWITH } { PAIR ; PAIR ; NIL operation ; PAIR } }
+          { FAILWITH } }
+".
+
