src/contracts_coq/did_manager_string.v
@@ -2,8 +2,8 @@ Require Import String.
 
 Definition did_manager_string : string := "
 { parameter
-    (or (or (address %rotateAuthentication) (address %rotateOwner))
-        (pair %rotateService (string %endpoint) (string %type_))) ;
+    (or (address %owner)
+        (or (address %auth) (pair %service (string %endpoint) (string %type_)))) ;
   storage
     (pair (pair (big_map %metadata string bytes) (address %owner))
           (pair (pair %service (string %endpoint) (string %type_))
@@ -24,6 +24,25 @@ Definition did_manager_string : string := "
          GT ;
          IF { PUSH string ""Tez not accepted."" ; FAILWITH } {} ;
          IF_LEFT
+           { SWAP ;
+             DUP ;
+             DUG 2 ;
+             CDR ;
+             CDR ;
+             DIG 2 ;
+             DUP ;
+             DUG 3 ;
+             CDR ;
+             CAR ;
+             PAIR ;
+             SWAP ;
+             DIG 2 ;
+             CAR ;
+             CAR ;
+             PAIR ;
+             PAIR ;
+             NIL operation ;
+             PAIR }
            { IF_LEFT
                { SWAP ;
                  DUP ;
@@ -48,38 +67,19 @@ Definition did_manager_string : string := "
                  DUG 2 ;
                  CDR ;
                  CDR ;
-                 DIG 2 ;
-                 DUP ;
-                 DUG 3 ;
-                 CDR ;
-                 CAR ;
+                 SWAP ;
                  PAIR ;
                  SWAP ;
+                 DUP ;
+                 DUG 2 ;
+                 CAR ;
+                 CDR ;
                  DIG 2 ;
                  CAR ;
                  CAR ;
                  PAIR ;
                  PAIR ;
                  NIL operation ;
-                 PAIR } }
-           { SWAP ;
-             DUP ;
-             DUG 2 ;
-             CDR ;
-             CDR ;
-             SWAP ;
-             PAIR ;
-             SWAP ;
-             DUP ;
-             DUG 2 ;
-             CAR ;
-             CDR ;
-             DIG 2 ;
-             CAR ;
-             CAR ;
-             PAIR ;
-             PAIR ;
-             NIL operation ;
-             PAIR } } }
+                 PAIR } } } }
 ".
 
